AwsCryptographyPrimitives/runtimes/java/src/main/smithy-generated/software/amazon/cryptography/primitives/model/KdfCtrDeriveInput.java
@@ -1,0 +1,111 @@
+// Copyright Amazon.com Inc. or its affiliates. All Rights Reserved.
+// SPDX-License-Identifier: Apache-2.0
+// Do not modify this file. This file is machine generated, and any changes to it will be overwritten.
+package software.amazon.cryptography.primitives.model;
+
+import java.nio.ByteBuffer;
+import java.util.Objects;
+
+public class KdfCtrDeriveInput {
+  private final HMacInput macAlgorithm;
+
+  private final ByteBuffer iv;
+
+  private final ByteBuffer ikm;
+
+  protected KdfCtrDeriveInput(BuilderImpl builder) {
+    this.macAlgorithm = builder.macAlgorithm();
+    this.iv = builder.iv();
+    this.ikm = builder.ikm();
+  }
+
+  public HMacInput macAlgorithm() {
+    return this.macAlgorithm;
+  }
+
+  public ByteBuffer iv() {
+    return this.iv;
+  }
+
+  public ByteBuffer ikm() {
+    return this.ikm;
+  }
+
+  public Builder toBuilder() {
+    return new BuilderImpl(this);
+  }
+
+  public static Builder builder() {
+    return new BuilderImpl();
+  }
+
+  public interface Builder {
+    Builder macAlgorithm(HMacInput macAlgorithm);
+
+    HMacInput macAlgorithm();
+
+    Builder iv(ByteBuffer iv);
+
+    ByteBuffer iv();
+
+    Builder ikm(ByteBuffer ikm);
+
+    ByteBuffer ikm();
+
+    KdfCtrDeriveInput build();
+  }
+
+  static class BuilderImpl implements Builder {
+    protected HMacInput macAlgorithm;
+
+    protected ByteBuffer iv;
+
+    protected ByteBuffer ikm;
+
+    protected BuilderImpl() {
+    }
+
+    protected BuilderImpl(KdfCtrDeriveInput model) {
+      this.macAlgorithm = model.macAlgorithm();
+      this.iv = model.iv();
+      this.ikm = model.ikm();
+    }
+
+    public Builder macAlgorithm(HMacInput macAlgorithm) {
+      this.macAlgorithm = macAlgorithm;
+      return this;
+    }
+
+    public HMacInput macAlgorithm() {
+      return this.macAlgorithm;
+    }
+
+    public Builder iv(ByteBuffer iv) {
+      this.iv = iv;
+      return this;
+    }
+
+    public ByteBuffer iv() {
+      return this.iv;
+    }
+
+    public Builder ikm(ByteBuffer ikm) {
+      this.ikm = ikm;
+      return this;
+    }
+
+    public ByteBuffer ikm() {
+      return this.ikm;
+    }
+
+    public KdfCtrDeriveInput build() {
+      if (Objects.isNull(this.macAlgorithm()))  {
+        throw new IllegalArgumentException("Missing value for required field `macAlgorithm`");
+      }
+      if (Objects.isNull(this.ikm()))  {
+        throw new IllegalArgumentException("Missing value for required field `ikm`");
+      }
+      return new KdfCtrDeriveInput(this);
+    }
+  }
+}
