AwsCryptographyPrimitives/src/KDF/KdfCtr.dfy
@@ -1,0 +1,135 @@
+// Copyright Amazon.com Inc. or its affiliates. All Rights Reserved.
+// SPDX-License-Identifier: Apache-2.0
+
+include "../HKDF/HMAC.dfy"
+include "../Digest.dfy"
+include "../../Model/AwsCryptographyPrimitivesTypes.dfy"
+
+/*
+ * Implementation of the https://nvlpubs.nist.gov/nistpubs/SpecialPublications/NIST.SP.800-108r1.pdf
+ * Key Derivation in Counter Mode Using Pseudorandom Functions
+ */
+module KdfCtr {
+  import opened StandardLibrary
+  import opened Wrappers
+  import opened UInt = StandardLibrary.UInt
+  import UTF8
+  import Types = AwsCryptographyPrimitivesTypes
+  import HMAC
+  import Digest
+
+  const SEPARATION_INDICATOR: seq<uint8> := [0x00];
+  const COUNTER_START_VALUE: uint32 := 1;
+
+  // This implementation of te spec is restricted to only deriving
+  // 32 bytes of key material. We will have to consider the effect of allowing different
+  // key length to the hierarchy keyring.
+  method KdfCounterMode(input: Types.KdfCtrInput)
+    returns (output: Result<seq<uint8>, Types.Error>)
+    ensures output.Success? ==> |output.value| == input.expectedLength as nat
+  {
+    :- Need(
+      // Although KDF can support multiple digests; for our use case we only want
+      // to use SHA 256; we may rethink this if we ever want to support other algorithms
+      // We are requiring the requested length to be 32 bytes since this is only used for the hierarchy
+      // keyring it requires to derive a 32 byte key.
+      && input.digestAlgorithm == Types.DigestAlgorithm.SHA_256
+      && |input.ikm| == 32
+      && input.nonce.Some?
+      && |input.nonce.value| == 16 
+      && input.expectedLength == 32
+      && 0 < ((input.expectedLength as int) * 8) as int < INT32_MAX_LIMIT,
+      Types.AwsCryptographicPrimitivesError(message := "Kdf in Counter Mode input is invalid.")
+    );
+    
+    var ikm := input.ikm;
+    var label_ := input.purpose.UnwrapOr([]);
+    var info := input.nonce.UnwrapOr([]);
+    var okm := [];
+
+    // Compute length in bits of the input going into the PRF.
+    var internalLength : uint32 := (4 + |SEPARATION_INDICATOR| + 4) as uint32;
+    :- Need(
+      && internalLength as int + |label_| + |info| < INT32_MAX_LIMIT, 
+      Types.AwsCryptographicPrimitivesError(message:= "Input Length exceeds INT32_MAX_LIMIT")
+    );
+
+    // Compute length in bits of the output from the PRF. "L" in SP800-108.
+    var lengthBits : seq<uint8> := UInt.UInt32ToSeq((input.expectedLength * 8) as uint32);
+    var explicitInfo := label_ + SEPARATION_INDICATOR + info + lengthBits;
+
+    :- Need(
+      4 + |explicitInfo| < INT32_MAX_LIMIT,
+      Types.AwsCryptographicPrimitivesError(message := "PRF input length exceeds INT32_MAX_LIMIT.")
+    );
+
+    okm :- RawDerive(ikm, explicitInfo, input.expectedLength, 0);
+
+    return Success(okm);
+  }
+
+  method RawDerive(ikm: seq<uint8>, explicitInfo: seq<uint8>, length: int32, offset: int32)
+    returns (output: Result<seq<uint8>, Types.Error>)
+    requires 
+      && |ikm| == 32
+      && length == 32
+      && 4 + |explicitInfo| < INT32_MAX_LIMIT
+      && length as int + Digest.Length(Types.DigestAlgorithm.SHA_256) < INT32_MAX_LIMIT - 1
+    ensures output.Success? ==> |output.value| == length as int
+  {
+    // We will only support HMAC_SHA256, so no need to support additional Digests
+    var derivationMac := Types.DigestAlgorithm.SHA_256;
+    var hmac :- HMAC.HMac.Build(derivationMac);
+    hmac.Init(key := ikm);
+
+    var macLengthBytes := Digest.Length(derivationMac) as int32; // "h" in SP800-108
+    // Number of iterations required to compose output of required length.
+    var iterations := ((length + macLengthBytes) + 1) / macLengthBytes; // "n" in SP800-108
+    var buffer := [];
+
+    // Counter "i"
+    var i : seq<uint8> := UInt.UInt32ToSeq(COUNTER_START_VALUE);
+
+    for iteration := 1 to iterations + 1
+      invariant |i| == 4
+      invariant hmac.GetKey() == ikm
+    {
+      /*
+       * SP800-108 defines PRF(s,x), the "x" variable is prfInput below.
+       */
+      // i || label || 0x00 || context (info) || L
+      hmac.Update(i);
+      hmac.Update(explicitInfo);
+      var tmp := hmac.GetResult();
+      buffer := buffer + tmp;
+
+      i := Increment(i);
+    }
+
+    :- Need(
+      |buffer| >= length as int,
+      Types.AwsCryptographicPrimitivesError(message := "Failed to derive key of requested length")
+    );
+
+    return Success(buffer[..length]);
+  }
+  
+  function method Increment(x : seq<uint8>) : (ret : seq<uint8>)
+    requires |x| == 4
+    ensures |ret| == 4
+  {
+    // increments the counter x which represents the number of iterations
+    // as a bit sequence
+    if x[3] < 255 then
+      [x[0], x[1], x[2], x[3]+1]
+    else if x[2] < 255 then
+      [x[0], x[1], x[2]+1, 0]
+    else if x[1] < 255 then
+      [x[0], x[1]+1, 0, 0]
+    else if x[0] < 255 then
+      [x[0]+1, 0, 0, 0]
+    else
+      [0, 0, 0, 0]
+  }
+
+}
